fix CRLF and WIP to integrate Data/Mem changes

src/Dafny/llvm.i.dfy
@@ -1,34 +1,27 @@
 include "ops.dfy"
 include "types.dfy"
-include "simpleMemory.i.dfy"
-include "typeConversions.i.dfy"
+include "memory.dfy"
+// include "typeConversions.i.dfy"
 
 module LLVM_def {
 
     import opened types
     import opened ops
-    import opened simple_memory
-    import opened type_conversion
+    import opened memory
+    // import opened type_conversion
 
     type addr = int
     type LocalVar = string
     type GlobalVar = string
 
     datatype state = State(
-        lvs:map<LocalVar, Value>,
-        gvs:map<GlobalVar, Value>,
-        m:memmap,
+        lvs:map<LocalVar, Data>,
+        gvs:map<GlobalVar, Data>,
+        m:MemState,
         ok:bool)
 
-    // Taken from Vale -- modify for llvm
-    type shift_amount = s | 0 <= s < 32 // Some shifts allow s=32, but we'll be conservative for simplicity
-    datatype Shift =
-        | LSLShift(amount_lsl:shift_amount)
-        | LSRShift(amount_lsr:shift_amount)
-        | RORShift(amount_ror:shift_amount)
 
-
-    datatype operand = Val(v:Value) | LV(l:LocalVar) | GV(g:GlobalVar)
+    datatype operand = D(d:Data) | LV(l:LocalVar) | GV(g:GlobalVar)
     datatype condition = eq | ne | ugt | uge | ult | ule | sgt | sge | slt | sle
 
     //---
@@ -37,17 +30,17 @@ module LLVM_def {
     //-----------------------------------------------------------------------------
 
     datatype ins =
-    | ADD(dst:operand, src1ADD:operand, src2ADD:operand)
-    | SUB(dst:operand, src1ADD:operand, src2ADD:operand)
+    | ADD(dst:operand, t:IntType, src1ADD:operand, src2ADD:operand)
+    | SUB(dst:operand, t:IntType, src1SUB:operand, src2SUB:operand)
     | BR(flag:bool, labelTrue:string,labelFalse:string)
     | CALL() //needs work
-    | GETELEMENTPTR(t:operand,p:ptr) //needs work VV
-    | ICMP(cond:condition,t:operand,src1:operand,src2:operand)
+    | GETELEMENTPTR() //needs work VV
+    | ICMP(cond:condition,dst:operand,src1:operand,src2:operand)
     | RET()
-    | ZEXT(dst:operand,t0:Value,src:operand,t1:Value)
+    | ZEXT(dst:operand,tSrc:IntType,src:operand,tDst:IntType)
     | SHL()
     | TRUN()
-    | SEXT(dst:operand,t0:Value,src:operand,t1:Value)
+    | SEXT(dst:operand,tSrc:IntType,src:operand,tDst:IntType)
     
 
 
@@ -56,10 +49,10 @@ module LLVM_def {
         s.ok 
         && |s.lvs| == 0
         && |s.gvs| == 0
-        && ValidMemState(s.m)    
+        && MemInit(s.m)    
     }
 
-    predicate{:opaque} ValidRegState(lvs:map<LocalVar, Value>,gvs:map<GlobalVar, Value>)
+    predicate{:opaque} ValidRegState(lvs:map<LocalVar, Data>,gvs:map<GlobalVar, Data>)
     {
         forall l:LocalVar :: l in lvs && forall g:GlobalVar :: g in gvs
     }
@@ -67,13 +60,13 @@ module LLVM_def {
     predicate ValidState(s:state)
     
     {
-        ValidRegState(s.lvs,s.gvs) && ValidMemState(s.m)
+        ValidRegState(s.lvs,s.gvs) && MemValid(s.m)
     }
 
     predicate ValidOperand(s:state,o:operand)
     {
         match o
-            case Val(v) => true
+            case D(d) => true
             case LV(l) => l in s.lvs
             case GV(g) => g in s.gvs
     }
@@ -81,39 +74,41 @@ module LLVM_def {
     predicate ValidInstruction(s:state, ins:ins)
     {
         ValidState(s) && match ins
-            case ADD(t,src1,src2) => ValidOperand(s,t) && ValidOperand(s,src1) && ValidOperand(s,src2)
-                                    && numericalValue(OperandContents(s,t)) &&  numericalValue(OperandContents(s,src1)) && numericalValue(OperandContents(s,src2))
-                                    && matchOps(OperandContents(s,t),OperandContents(s,src1),OperandContents(s,src2))
-            case SUB(t,src1,src2) => ValidOperand(s,t) && ValidOperand(s,src1) && ValidOperand(s,src2) 
-                                    && numericalValue(OperandContents(s,t)) &&  numericalValue(OperandContents(s,src1)) && numericalValue(OperandContents(s,src2))
-                                    && matchOps(OperandContents(s,t),OperandContents(s,src1),OperandContents(s,src2))
+            case ADD(dst,t,src1,src2) => && ValidOperand(s,dst) && ValidOperand(s,src1) && ValidOperand(s,src2)
+                                         && isInt(OperandContents(s,src1)) && isInt(OperandContents(s,src2))
+                                         && intTypesMatch(OperandContents(s,src1),OperandContents(s,src2))
+            case SUB(dst,t,src1,src2) => && ValidOperand(s,dst) && ValidOperand(s,src1) && ValidOperand(s,src2) 
+                                         && isInt(OperandContents(s,src1)) && isInt(OperandContents(s,src2))
+                                         && intTypesMatch(OperandContents(s,src1),OperandContents(s,src2))
             case BR(cond, labelTrue,labelFalse) => true
             case CALL() => true
-            case GETELEMENTPTR(t,p) => true
+            case GETELEMENTPTR() => true
             case ICMP(cond,dst,src1,src2) => ValidOperand(s,dst) && ValidOperand(s,src1) && ValidOperand(s,src2) 
             case RET() => true
-            case ZEXT(dst,t0,src,t1) => ValidOperand(s,dst) && ValidOperand(s,src) && typesMatch(t0,OperandContents(s,src)) 
-                                        && unsignedVal(t0) && unsignedVal(t1) && unsignedValLT(t0,t1) 
+            case ZEXT(dst,tSrc,src,tDst) => && ValidOperand(s,dst) && ValidOperand(s,src) && isInt(OperandContents(s,src))
+                                            && tSrc == OperandContents(s,src).itype 
+                                            && !tSrc.signed && !tDst.signed && tSrc.size <= tDst.size
             case SHL() => true
             case TRUN() => true
-            case SEXT(dst,t0,src,t1) => ValidOperand(s,dst) && ValidOperand(s,src) && typesMatch(t0,OperandContents(s,src)) 
-                                        && signedVal(t0) && signedVal(t1) && signedValLT(t0,t1) 
+            case SEXT(dst,tSrc,src,tDst) => && ValidOperand(s,dst) && ValidOperand(s,src) && isInt(OperandContents(s,src))
+                                        && tSrc == OperandContents(s,src).itype 
+                                        && tSrc.signed && tDst.signed && tSrc.size <= tDst.size
                  
     }
 
-    predicate matchOps(v0:Value,v1:Value,v2:Value)
-    {
-        (v0.Val8? ==> v1.Val8? && v2.Val8?)
-        && (v0.Val16? ==> v1.Val16? && v2.Val16?)
-        && (v0.Val32? ==> v1.Val32? && v2.Val32?)
-        && (v0.Val64? ==> v1.Val64? && v2.Val64?)
-        && (v0.ValBool? ==> !v1.ValBool? && !v2.ValBool?)
-    }
+    // predicate matchOps(v0:Value,v1:Value,v2:Value)
+    // {
+    //     (v0.Val8? ==> v1.Val8? && v2.Val8?)
+    //     && (v0.Val16? ==> v1.Val16? && v2.Val16?)
+    //     && (v0.Val32? ==> v1.Val32? && v2.Val32?)
+    //     && (v0.Val64? ==> v1.Val64? && v2.Val64?)
+    //     && (v0.ValBool? ==> !v1.ValBool? && !v2.ValBool?)
+    // }
 
-     predicate numericalValue(v:Value)
-    {
-        v.Val8? || v.Val16? || v.Val32? || v.Val64?
-    }
+    //  predicate numericalValue(v:Value)
+    // {
+    //     v.Val8? || v.Val16? || v.Val32? || v.Val64?
+    // }
 
     //EVAL//
     predicate ValidRegOperand(s:state, o:operand)
@@ -121,30 +116,30 @@ module LLVM_def {
         ValidOperand(s,o)
     }
 
-    function OperandContents(s:state, o:operand): Value
+    function OperandContents(s:state, o:operand): Data
         requires ValidOperand(s,o)
         requires ValidState(s)
     {
 
         reveal_ValidRegState();
         match o
-            case Val(v) => v
+            case D(d) => d
             case LV(l) => s.lvs[l]
             case GV(g) => s.gvs[g]
            
     }
 
 
-    predicate evalUpdate(s:state, o:operand, val:Value, r:state)
+    predicate evalUpdate(s:state, o:operand, data:Data, r:state)
         requires ValidState(s)
         requires ValidRegOperand(s,o)
-        ensures evalUpdate(s, o, val, r) ==> ValidState(r)
+        ensures evalUpdate(s, o, data, r) ==> ValidState(r)
     {
         reveal_ValidRegState();
         match o
-            case Val(v) => r == s 
-            case GV(g) => r == s.(gvs := s.gvs[g := val]) 
-            case LV(l) => r == s.(lvs := s.lvs[l := val]) 
+            case D(d) => r == s 
+            case GV(g) => r == s.(gvs := s.gvs[g := data]) 
+            case LV(l) => r == s.(lvs := s.lvs[l := data]) 
             
     }
 
@@ -152,70 +147,96 @@ module LLVM_def {
     {   
         if !s.ok || !ValidInstruction(s, ins) then !r.ok
         else match ins
-            case ADD(t,src1,src2) => evalUpdate(s, t, 
-                                evalADD(OperandContents(s,t),OperandContents(s,src1),OperandContents(s,src2)),r)
-            case SUB(t,src1,src2) => evalUpdate(s, t, 
-                                evalSUB(OperandContents(s,t),OperandContents(s,src1),OperandContents(s,src2)),r)
-            case BR(cond, labelTrue,labelFalse) => true
+            case ADD(dst,t,src1,src2) => evalUpdate(s, dst, 
+                                evalADD(t,OperandContents(s,src1),OperandContents(s,src2)),r)
+            case SUB(dst,t,src1,src2) => evalUpdate(s, dst, 
+                                evalSUB(t,OperandContents(s,src1),OperandContents(s,src2)),r)
             case CALL() => true
-            case GETELEMENTPTR(t,p) => true
-            case ICMP(cond,dst,src1,src2) => evalUpdate(s, dst, 
-                                ValBool(evalICMP(cond,OperandContents(s,dst),OperandContents(s,src1),OperandContents(s,src2))),r)
+            case GETELEMENTPTR() => true
+            // case ICMP(cond,dst,src1,src2) => evalUpdate(s, dst, 
+            //                     ValBool(evalICMP(cond,OperandContents(s,dst),OperandContents(s,src1),OperandContents(s,src2))),r)
             case RET() => true
-            case ZEXT(dst,t0,src,t1) => evalUpdate(s, dst, 
-                                  evalZEXT(t0,OperandContents(s,src),t1),r)
+            case BR(cond, labelTrue,labelFalse) => true
+
+            // case ZEXT(dst,t0,src,t1) => evalUpdate(s, dst, 
+            //                       evalZEXT(t0,OperandContents(s,src),t1),r)
             case SHL() => true
             case TRUN() => true
-            case SEXT(dst,t0,src,t1) => true
+            // case SEXT(dst,t0,src,t1) => true
+            case SEXT(dst,tSrc,src,tDst) => true
+            case ZEXT(dst,tSrc,src,tDst) => true
+            case ICMP(cond,dst,src1,src2) => true
     }
 
 
 
 
-    function evalADD(v0:Value,v1:Value,v2:Value): Value
-        requires numericalValue(v0);
-        requires numericalValue(v1);
-        requires numericalValue(v2);
-        requires matchOps(v0,v1,v2)
+    function evalADD(t:IntType_,v0:Data,v1:Data): Data
+        requires isInt(v0)
+        requires isInt(v1)
+        requires intTypesMatch(v0,v1)
+    { 
+
+        if v0.itype == IntType(1, false) then UInt8(BitwiseAdd8(DataToUInt8(v0),DataToUInt8(v1))) else 
+        if v0.itype == IntType(2, false) then UInt16(BitwiseAdd16(DataToUInt16(v0),DataToUInt16(v1))) else 
+        if v0.itype == IntType(4, false) then UInt32(BitwiseAdd32(DataToUInt32(v0),DataToUInt32(v1))) else 
+        if v0.itype == IntType(8, false) then UInt64(BitwiseAdd64(DataToUInt64(v0),DataToUInt64(v1))) else
+        if v0.itype == IntType(1, true) then SInt8(BitwiseSAdd8(DataToSInt8(v0),DataToSInt8(v1))) else 
+        if v0.itype == IntType(2, true) then SInt16(BitwiseSAdd16(DataToSInt16(v0),DataToSInt16(v1))) else 
+        if v0.itype == IntType(4, true) then SInt32(BitwiseSAdd32(DataToSInt32(v0),DataToSInt32(v1))) else 
+        if v0.itype == IntType(8, true) then SInt64(BitwiseSAdd64(DataToSInt64(v0),DataToSInt64(v1))) else v0
+       
+    }
+
+
+
+
+    function evalSUB(t:IntType_,v0:Data,v1:Data): Data
+        requires isInt(v0)
+        requires isInt(v1)
+        requires intTypesMatch(v0,v1)
     {
-       if v0.Val8? then Val8(BitwiseAdd8(ValueContents8Bit(v1),ValueContents8Bit(v2))) else 
-       if v0.Val16? then Val16(BitwiseAdd16(ValueContents16Bit(v1),ValueContents16Bit(v2))) else
-       if v0.Val32? then Val32(BitwiseAdd32(ValueContents32Bit(v1),ValueContents32Bit(v2))) else
-       if v0.Val64? then Val64(BitwiseAdd64(ValueContents64Bit(v1),ValueContents64Bit(v2))) else
-                        Val8(0)
+        if v0.itype == IntType(1, false) then UInt8(BitwiseSub8(DataToUInt8(v0),DataToUInt8(v1))) else 
+        if v0.itype == IntType(2, false) then UInt16(BitwiseSub16(DataToUInt16(v0),DataToUInt16(v1))) else 
+        if v0.itype == IntType(4, false) then UInt32(BitwiseSub32(DataToUInt32(v0),DataToUInt32(v1))) else 
+        if v0.itype == IntType(8, false) then UInt64(BitwiseSub64(DataToUInt64(v0),DataToUInt64(v1))) else
+        if v0.itype == IntType(1, true) then SInt8(BitwiseSSub8(DataToSInt8(v0),DataToSInt8(v1))) else 
+        if v0.itype == IntType(2, true) then SInt16(BitwiseSSub16(DataToSInt16(v0),DataToSInt16(v1))) else 
+        if v0.itype == IntType(4, true) then SInt32(BitwiseSSub32(DataToSInt32(v0),DataToSInt32(v1))) else 
+        if v0.itype == IntType(8, true) then SInt64(BitwiseSSub64(DataToSInt64(v0),DataToSInt64(v1))) else v0
     }
 
-    function evalSUB(v0:Value,v1:Value,v2:Value): Value
-        requires numericalValue(v0);
-        requires numericalValue(v1);
-        requires numericalValue(v2);
-        requires matchOps(v0,v1,v2)
+    // function evalSUB(v0:Value,v1:Value,v2:Value): Value
+    //     requires numericalVisIntalue(v0);
+    //     requires isInt(v1);
+    //     requires isInt(v2);
+    //     requires matchOps(v0,v1,v2)
         
-    {
-       if v0.Val8? then Val8(BitwiseSub8(ValueContents8Bit(v1),ValueContents8Bit(v2))) else 
-       if v0.Val16? then Val16(BitwiseSub16(ValueContents16Bit(v1),ValueContents16Bit(v2))) else
-       if v0.Val32? then Val32(BitwiseSub32(ValueContents32Bit(v1),ValueContents32Bit(v2))) else
-       if v0.Val64? then Val64(BitwiseSub64(ValueContents64Bit(v1),ValueContents64Bit(v2))) else
-                        Val8(0)
-    }
+    // {
+    //    if v0.Val8? then Val8(BitwiseSub8(ValueContents8Bit(v1),ValueContents8Bit(v2))) else 
+    //    if v0.Val16? then Val16(BitwiseSub16(ValueContents16Bit(v1),ValueContents16Bit(v2))) else
+    //    if v0.Val32? then Val32(BitwiseSub32(ValueContents32Bit(v1),ValueContents32Bit(v2))) else
+    //    if v0.Val64? then Val64(BitwiseSub64(ValueContents64Bit(v1),ValueContents64Bit(v2))) else
+    //                     Val8(0)
+    // }
 
 // eq | ne | ugt | uge | ult | ule | sgt | sge | slt | sle
 
-    function evalICMP(c:condition,t:Value,v0:Value,v1:Value): bool
-        // requires matchOps(t,v0,v1)
-    {
-        match c
-            case eq => v0 == v1
-            case ne => v0 != v1
-            case ugt => v0 > v1
-            case uge => v0 > v1 || v0 == v1
-            case ult => v0 < v1
-            case ule => v0 < v1 || v0 == v1
-            case sgt => true // signed 
-            case sge => true // signed 
-            case slt => true // signed 
-            case sle => true // signed 
-    }
+    // function evalICMP(c:condition,t:Value,v0:Value,v1:Value): bool
+    //     // requires matchOps(t,v0,v1)
+    // {
+    //     match c
+    //         case eq => v0 == v1
+    //         case ne => v0 != v1
+    //         case ugt => v0 > v1
+    //         case uge => v0 > v1 || v0 == v1
+    //         case ult => v0 < v1
+    //         case ule => v0 < v1 || v0 == v1
+    //         case sgt => true // signed 
+    //         case sge => true // signed 
+    //         case slt => true // signed 
+    //         case sle => true // signed 
+    // }
 
 
     
